update

Lexi.v
@@ -11,55 +11,62 @@ Open Scope Lexi_scope.
    ------------ ------------ ------------
    ------------ ------------ ------------ *)
 Inductive variable := 
-  | dbjind_var : nat -> variable
-  | free_var : var -> variable.
+| dbjind_var : nat -> variable
+| free_var : var -> variable.
 Inductive code_label := c_lab : string -> code_label.
 Inductive obj_label := obj_lab : string -> obj_label.
 Inductive hdl_label := hdl_lab : string -> hdl_label.
 Inductive data_label : Type := 
-  | obj_data_lab : obj_label -> data_label
-  | hdl_data_lab : hdl_label -> data_label.
+| obj_data_lab : obj_label -> data_label
+| hdl_data_lab : hdl_label -> data_label.
 Inductive static_const : Type :=
-  | nat_const : nat -> static_const
-  | c_lab_const : code_label -> static_const.
+| nat_const : nat -> static_const
+| c_lab_const : code_label -> static_const.
 Inductive runtime_const : Type :=
-  | run_const : static_const -> runtime_const
-  | d_lab_const : data_label -> runtime_const
-  | ns.
+| run_const : static_const -> runtime_const
+| d_lab_const : data_label -> runtime_const
+| ns.
 Inductive value :=
-  | const_val : static_const -> value
-  | var_val : variable -> value.
+| const_val : static_const -> value
+| var_val : variable -> value.
 Definition local_env : Type := list runtime_const.
 Inductive annotation : Type :=
-  | tail
-  | abort
-  | general.
+| tail
+| abort
+| general.
 Inductive expr : Type :=
-  | val_e : value -> expr
-  | add : value -> value -> expr
-  | newref : list value -> expr
-  | pi : nat -> value -> expr
-  | asgn : value -> nat -> value -> expr
-  | app : value -> (list value) -> expr
-  | handle : code_label -> code_label -> annotation -> value -> expr
-  | raise : annotation -> value -> value -> expr
-  | resume : value -> value -> expr
-  | exit : value -> expr
+| val_e : value -> expr
+| add : value -> value -> expr
+| newref : list value -> expr
+| pi : nat -> value -> expr
+| asgn : value -> nat -> value -> expr
+| app : value -> (list value) -> expr
+| handle : code_label -> code_label
+           -> annotation -> value -> expr
+| raise : annotation -> value -> value -> expr
+| resume : value -> value -> expr
+| exit : value -> expr
 with term : Type :=
-  | val_term : value -> term
-  | bind : expr -> term -> term
-  | halt
-with a_frame: Type := act_f : local_env -> term -> a_frame
-with h_frame : Type := handler_f : hdl_label -> hdl_label ->
-    code_label -> annotation -> h_frame
+| val_term : value -> term
+| bind : expr -> term -> term
+| halt
+with a_frame: Type :=
+  act_f : local_env -> term -> a_frame
+with h_frame : Type :=
+  handler_f : hdl_label -> hdl_label ->
+              code_label -> annotation -> h_frame
 with frame : Type :=
-  | h_f : h_frame -> frame
-  | a_f : a_frame -> frame
-with heap_const : Type :=
-  | tuple : list runtime_const -> heap_const
-  | cont : list frame -> heap_const.
+| h_f : h_frame -> frame
+| a_f : a_frame -> frame
+with heap_cont : Type :=
+| cont : list frame -> heap_cont
+| empty_cont.
+Inductive heap_tuple : Type :=
+| tuple : list runtime_const -> heap_tuple.
 Definition eval_context := list frame.
-Definition heap := obj_label -> heap_const.
+Definition tup_heap := obj_label -> heap_tuple.
+Definition cont_heap := obj_label -> heap_cont.
+Definition heap := (tup_heap * cont_heap)%type.
 Inductive function : Type :=
   func : nat -> term -> function.
 Definition code : Type := code_label -> function.
@@ -90,16 +97,23 @@ Coercion a_f : a_frame >-> frame.
               Map Related Helpers
    -------------------------------------------- *)
 (* Heap *)
-Definition empty_hconst := tuple nil.
+Definition empty_tup := tuple nil.
 Definition h_eqb (a b : obj_label) := 
   match a,b with
   | obj_lab a', obj_lab b' => String.eqb a' b'
   end.
-Definition h_empty : heap := fun _ => empty_hconst.
-Definition h_update (m : heap) (x : obj_label) (v : heap_const) :=
+Definition th_empty : tup_heap := fun _ => empty_tup.
+Definition ch_empty : cont_heap := fun _ => empty_cont.
+Definition h_empty : heap := (th_empty,ch_empty).
+Definition th_update (m : tup_heap) (x : obj_label) (v : heap_tuple) :=
   fun x' => if h_eqb x x' then v else m x'.
-Notation "x '!->h' v ';' m" := (h_update m x v)
+Notation "x '!->t' v ';' m" := (th_update m x v)
   (at level 100, v at next level, right associativity):Lexi_scope.
+Definition ch_update (m : cont_heap) (x : obj_label) (v : heap_cont) :=
+  fun x' => if h_eqb x x' then v else m x'.
+Notation "x '!->ch' v ';' m" :=
+  (ch_update m x v)
+    (at level 100, v at next level, right associativity):Lexi_scope.
 
 (* Environment *)
 Definition env_fetch (env: local_env) (var:variable)
@@ -139,7 +153,7 @@ Definition var_deref (E:local_env) (val:value)
   end.
 
 (* --------------------------------------------
-                      Interpreter
+               Operational Semantics
    -------------------------------------------- *)
 (* We assume that code is already initialized.
    Initialization is defined separately later. 
@@ -154,21 +168,21 @@ Inductive step (C:code) : (heap * eval_context * local_env * term)
       (H,K,(run_const (i1+i2)) :: E,t)
   | L_value : forall H K E t (v:value),
     step C (H,K,E, bind v t) (H,K,(var_deref E v) :: E,t)
-  | L_new : forall H K E t (lst:list value) (L:obj_label),
-    H L = empty_hconst ->
-    step C (H,K,E, bind (newref lst) t)
-      (L !->h tuple (List.map (var_deref E) lst); H, K, (d_lab_const L) :: E, t)
-  | L_get : forall H K E t (i:nat) (v:value)
+  | L_new : forall tH cH K E t (lst:list value) (L:obj_label),
+    tH L = empty_tup ->
+    step C (tH,cH,K,E, bind (newref lst) t)
+      (L !->t tuple (List.map (var_deref E) lst); tH,cH, K, (d_lab_const L) :: E, t)
+  | L_get : forall tH cH K E t (i:nat) (v:value)
     (L:obj_label) (lst:list runtime_const),
-    var_deref E v = L -> H L = tuple lst ->
-    step C (H,K,E, bind (pi i v) t)
-      (H,K,(nth (1+i) lst ns) :: E,t)
-  | L_set : forall H K E t (i:nat)
+    var_deref E v = L -> tH L = tuple lst ->
+    step C (tH,cH,K,E, bind (pi i v) t)
+      (tH,cH,K,(nth i lst ns) :: E,t) (* from (1+i) to i*)
+  | L_set : forall tH cH K E t (i:nat)
     (v v':value) (L:obj_label) (lst:list runtime_const),
-    var_deref E v = L -> H L = tuple lst ->
-    step C (H,K,E, bind (asgn v i v') t)
-      (L !->h tuple (update_nth (i-1) lst (var_deref E v')); H,
-      K,(var_deref E v') :: E,t)
+    var_deref E v = L -> tH L = tuple lst ->
+    step C (tH,cH,K,E, bind (asgn v i v') t)
+      (L !->t tuple (update_nth i lst (var_deref E v')); tH,
+      cH,K,(var_deref E v') :: E,t) (* from i-1 to i *)
   | L_handle : forall H K E t t'
     (v_env:value) (lst:list value) (A:annotation)
     (lab_body lab_op:code_label) (L L_env:hdl_label),
@@ -194,21 +208,21 @@ Inductive step (C:code) : (heap * eval_context * local_env * term)
   | L_ret : forall H K E E' t (v:value),
     step C (H,(a_f(act_f E t)) :: K,E',val_term v)
       (H,K,(var_deref E' v) :: E,t)
-  | L_raise : forall H K K' E t t' (v1 v2:value)
+  | L_raise : forall tH cH K K' E t t' (v1 v2:value)
     (L L_env:hdl_label) (L_k:obj_label) (L_y:data_label) (lab_op:code_label),
-    H L_k = empty_hconst -> var_deref E v1 = L ->
+    cH L_k = empty_cont -> var_deref E v1 = L ->
     C lab_op = func 3 t' -> var_deref E v2 = L_y ->
-    step C (H,K' ++ [h_f (handler_f L L_env lab_op general)] ++ K,E,
+    step C (tH,cH,K' ++ [h_f (handler_f L L_env lab_op general)] ++ K,E,
       bind (raise general v1 v2) t)
-      (L_k !->h 
+      (tH, L_k !->ch 
       cont ([a_f(act_f E t)] ++ K' ++ [h_f(handler_f L L_env lab_op general)]);
-      H,K,
+      cH,K,
       [d_lab_const L_k;d_lab_const L_y;d_lab_const L_env],t')
-  | L_resume : forall H K K' E E' t t' (v1 v2:value)
+  | L_resume : forall tH cH K K' E E' t t' (v1 v2:value)
     (L_k:obj_label),
-    var_deref E v1 = L_k -> H L_k = cont (a_f(act_f E' t') :: K') ->
-    step C (H,K,E,bind (resume v1 v2) t)
-      (L_k !->h tuple [ns]; H,
+    var_deref E v1 = L_k -> cH L_k = cont (a_f(act_f E' t') :: K') ->
+    step C (tH,cH,K,E,bind (resume v1 v2) t)
+      (tH, L_k !->ch empty_cont; cH,
       K' ++ [a_f(act_f E t)] ++ K,
       (var_deref E v2) :: E',t')
   | L_tailraise : forall H K K' E t t' (v1 v2:value)
@@ -232,3 +246,7 @@ Inductive step (C:code) : (heap * eval_context * local_env * term)
     step C (H,K,E,bind (exit v) t)
       (H,(a_f (act_f E t)) :: K,[var_deref E v],halt).
 Close Scope Lexi_scope.
+
+(* Changes made:
+
+Lexi heap now also starts index from 0 rather than 1. *)
