SimProof.v
@@ -1,4 +1,3 @@
-Set Implicit Arguments.
 Require Import Lists.List. Import ListNotations.
 Require Import Strings.String.
 From TLC Require Import LibLN.
@@ -6,6 +5,7 @@ From LSEH Require Import Lexi.
 From LSEH Require Import Salt.
 From LSEH Require Import LexiToSalt.
 From LSEH Require Import RelConfig.
+From LSEH Require Import Infrastructure.
 Module L := Lexi. Module S := Salt. Module LS := LexiToSalt.
 Module R := RelConfig.
 Delimit Scope Lexi_scope with L_scope.
@@ -26,118 +26,54 @@ Inductive multi_plus {X : Type} (R : X -> X -> Prop) : X -> X -> Prop :=
    ----------------------------------------------------------------- *)
 (* By Theorem 1 already proven, this is reduced to proving LS_rel satisfying
   the 3 conditions *)
-Ltac automation :=
-  subst; auto;repeat constructor;subst;try easy;
-  try discriminate;try congruence;try tauto.
 
-Definition fv_val (v : L.value) : vars :=
-  match v with
-  | var_val (free_var x) => \{x}
-  | var_val (dbjind_var i) => \{}
-  | const_val c => \{}
-  end.
-Fixpoint fv_vlst (vlst : list L.value) : vars :=
-  match vlst with
-  | [] => \{}
-  | v :: vlst' => (fv_val v) \u (fv_vlst vlst')
-  end.
-Definition fv_exp (exp : L.expr) : vars :=
-  match exp with
-  | L.val_e val => fv_val val
-  | L.add val1 val2 =>
-      (fv_val val1) \u (fv_val val2)
-  | L.newref val_lst => fv_vlst val_lst
-  | L.pi _ val => fv_val val
-  | L.asgn val1 _ val2 =>
-      (fv_val val1) \u (fv_val val2)
-  | L.app val val_lst => (fv_val val) \u (fv_vlst val_lst)
-  | L.handle _ _ _ val => fv_val val
-  | L.raise _ val1 val2 =>
-      (fv_val val1) \u (fv_val val2)
-  | L.resume val1 val2 =>
-      (fv_val val1) \u (fv_val val2)
-  | L.exit val => fv_val val
-  end.
-Fixpoint fv (tm : L.term) : vars :=
-  match tm with
-  | bind exp t => (fv_exp exp) \u (fv t)
-  | val_term v => (fv_val v)
-  | L.halt => \{}
-  end.
-(* ********************************************************************** *)
-(** ** Instantiation of tactics *)
-
-(** Tactic [gather_vars] returns a set of variables occurring in
-    the context of proofs, including domain of environments and
-    free variables in terms mentionned in the context. *)
-
-Ltac gather_vars :=
-  let A := gather_vars_with (fun x : vars => x) in
-  let B := gather_vars_with (fun x : var => \{x}) in
-  let C := gather_vars_with (fun x : L.value => fv_val x) in
-  let D := gather_vars_with (fun (x : list L.value) => fv_vlst x) in
-  let E := gather_vars_with (fun x : L.expr => fv_exp x) in
-  let F := gather_vars_with (fun x : L.term => fv x) in
-  constr:(A \u B \u C \u D \u E \u F).
-
-(** Tactic [pick_fresh x] adds to the context a new variable x
-    and a proof that it is fresh from all of the other variables
-    gathered by tactic [gather_vars]. *)
-
-Ltac pick_fresh Y :=
-  let L := gather_vars in (pick_fresh_gen L Y).
-
-(** Tactic [apply_fresh T as y] takes a lemma T of the form
-    [forall L ..., (forall x, x \notin L, P x) -> ... -> Q.]
-    instantiate L to be the set of variables occuring in the
-    context (by [gather_vars]), then introduces for the premise
-    with the cofinite quantification the name x as "y" (the second
-    parameter of the tactic), and the proof that x is not in L. *)
-
-Tactic Notation "apply_fresh" constr(T) "as" ident(x) :=
-  apply_fresh_base T gather_vars x.
-Tactic Notation "apply_fresh" constr(T) :=
-  apply_fresh_base T gather_vars ltac_no_arg.
-Hint Constructors lc_term L.step.
 
 Theorem cond1 : forall C1 C2 M1 M2 main_lab init_lab,
   code_trans C1 = C2 ->
   init_L (c_lab init_lab) (letrec C1 (bind (app (c_lab main_lab) [])
-    (bind (exit (var_val 1)) (val_term 0)))) M1
+    (bind (exit (var_val 0)) (val_term 0)))) M1
   -> init_S (cloc_str init_lab) (cloc_str main_lab) C2 M2 -> LS_rel M1 M2.
-Proof with automation.
+Proof with automate.
   intros. destruct M1 as [[[[LC LH] LK] LE] Lt], M2 as [[SC SH] SR].
   inversion H1... inversion H0...
   apply rel_LS with (len:=0) (Clab:=init_lab) (lst:=[])
     (SIlst:=[mov 0 (cloc main_lab 0); call 0;
-    push (reg_o 1); load 1 sp false 1; halt])
+    push (reg_o 1); load 1 sp false 0; halt])
     (Slsp:=hloc L_stack 0)...
   - destruct L_stack as [L_stack_str].
     apply rel_context with (Ks:=[]) (Flst:=[]) (E:=[])
       (s:=[]) (s':=[]) (s_out:=[]) (L_out:=L_stack_str) 
       (L_0:=L_stack_str)
       (H_stack:=sh_empty)...
-  - unfold S.c_update,S.c_eqb. rewrite eqb_refl...
-  - Admitted. (*apply_fresh lc_bind.
- as y. apply_fresh_base_simple bind_closed gather_vars. ltac_no_arg.*)
-(* TLC skipped *)
+  - intros. cbv in H. inversion H...
+  - unfold c_update. rewrite c_eqb_refl...
+  - repeat apply_fresh lc_bind...
+Qed.
 
 Theorem cond2 : forall M1 M2 i,
   LS_rel M1 M2 -> final_L M1 i -> final_S M2 i.
-Proof with automation.
+Proof with automate.
   intros. destruct M1 as [[[[LC LH] LK] LE] Lt], M2 as [[SC SH] SR].
   inversion H0... inversion H... inversion H10...
   simpl. rewrite H13. inversion H9... apply nth_middle.
 Qed.
 
-Definition stk_app f stk :=
+Definition un_tuple (tup:tuple_heap_val) : list word :=
+  match tup with tuple lst => lst end.
+Definition un_stack stk : list word :=
   match stk with
-  | stack lst => stack (f lst)
-  | no_stacks => no_stacks
+  | stack lst => lst
+  | no_stacks => []
   end.
+Lemma tuple_un_tuple : forall h_val,
+    tuple (un_tuple h_val) = h_val.
+Proof with automate. intros. destruct h_val... Qed.
+Lemma stack_un_stack : forall lst,
+    stack (un_stack (stack lst)) = stack lst.
+Proof with automate. intros... Qed.
 Lemma term_trans_not_nil : forall tm,
   term_trans tm <> [].
-Proof with automation.
+Proof with automate.
   intros. unfold not. destruct tm;simpl...
   destruct e;intros;simpl;apply eq_sym in H;
   generalize dependent H...
@@ -155,22 +91,125 @@ Theorem cond3 : forall LC SC H1 K1 E1 t1 R2 H2 H1' K1' E1' t1',
     multi_plus (S.step SC)
       (H2, R2) (H2', R2') /\
     LS_rel (LC, H1', K1', E1', t1') (SC, H2', R2')).
-Proof with automation.
+Proof with super_a.
   intros. inversion H... inversion H12...
-  inversion H0;automation;
+  inversion H0;automate;
   remember (List.map run_cst_trans E1 ++ s_out) as cur_stk_val;
   remember (cloc Clab (List.length lst)) as l;
   remember ((L_out,stack cur_stk_val)::H_stack) as cur_stkh.
   (* 14 stepping rules, prove the multi and rel for each *)
-  3:
-    { (* x = newref <v1,...,vn> *)
+  4:
+    { (* x = pi_i(v)*)
     destruct L as [L_str].
-    exists (cur_stkh,SH_cont,SH_tup
-      
-    
-  }
-  - (* x = v1 + v2 *) exists
-      ((L_out,stack ((int_w (i1+i2)) :: cur_stk_val))
+    exists ((L_out,
+              stack (run_cst_trans (nth i lst0 L.ns) :: cur_stk_val))
+              :: H_stack,SH_cont,SH_tup),
+      ([(ip,loc_w (incr_cloc 3 l));
+       (sp,loc_w (hloc L_out (1+(List.length cur_stk_val))));
+       (nat_reg 1,run_cst_trans (nth i lst0 L.ns));
+       (nat_reg 2,o2);(nat_reg 3,o3);(nat_reg 4,o4);
+        (nat_reg 5,o5);(nat_reg 6,o6)]). split.
+    (* stepping salt code for loading from heap *)
+    + apply multi_step with
+        (y:=((cur_stkh,SH_cont,SH_tup),
+              [(ip,loc_w (next_cloc l));
+               (sp,loc_w (hloc L_out (List.length cur_stk_val)));
+               (nat_reg 1,val_direct_trans v cur_stk_val);
+               (nat_reg 2,o2);(nat_reg 3,o3);(nat_reg 4,o4);
+               (nat_reg 5,o5);(nat_reg 6,o6)])).
+      { destruct v as [cst|[ind|str]].
+        - apply S_mov with
+            (d:=1) (o:=val_direct_trans (const_val cst) cur_stk_val) (l:=l)
+            (R:=[(ip,loc_w l);(sp,loc_w (hloc L_out (List.length cur_stk_val)));
+                 (nat_reg 1,o1);(nat_reg 2,o2);(nat_reg 3,o3);
+                 (nat_reg 4,o4);(nat_reg 5,o5);(nat_reg 6,o6)])
+            (H:=(cur_stkh,SH_cont,SH_tup)) (P:=SC)...
+        - pose proof S_load_stk as Ins. specialize Ins with
+          (d:=1) (s:=sp) (off:=ind)
+          (L:=L_out) (H_stk:=cur_stkh) (H_cont:=SH_cont)
+          (H_tup:=SH_tup) (sign:=false)
+          (lst:=cur_stk_val) (i:=List.length cur_stk_val)
+          (R:=[(ip,loc_w l);(sp,loc_w (hloc L_out (List.length cur_stk_val)));
+                 (nat_reg 1,o1);(nat_reg 2,o2);(nat_reg 3,o3);
+                 (nat_reg 4,o4);(nat_reg 5,o5);(nat_reg 6,o6)])
+          (l:=l) (P:=SC). rewrite PeanoNat.Nat.sub_diag in Ins.
+          apply Ins;automate;cbn.
+          + inversion H11. rewrite H15... apply nth_middle.
+          + rewrite h_eqb_refl...
+        - apply S_mov with
+            (d:=1) (o:=val_direct_trans (var_val str) cur_stk_val) (l:=l)
+            (R:=[(ip,loc_w l);(sp,loc_w (hloc L_out (List.length cur_stk_val)));
+                 (nat_reg 1,o1);(nat_reg 2,o2);(nat_reg 3,o3);
+                 (nat_reg 4,o4);(nat_reg 5,o5);(nat_reg 6,o6)])
+            (H:=(cur_stkh,SH_cont,SH_tup)) (P:=SC)... }
+      apply multi_step with
+        (y:=((cur_stkh,SH_cont,SH_tup),
+              [(ip,loc_w (incr_cloc 2 l));
+               (sp,loc_w (hloc L_out (List.length cur_stk_val)));
+               (nat_reg 1,run_cst_trans (nth i lst0 L.ns));
+               (nat_reg 2,o2);(nat_reg 3,o3);(nat_reg 4,o4);
+               (nat_reg 5,o5);(nat_reg 6,o6)])).
+      { pose proof S_load_tup as Temp. cbn in Temp.
+        specialize Temp with
+          (d:=1) (s:=nat_reg 1) (off:=i)
+          (L:=L_str) (H_stk:=cur_stkh) (H_cont:=SH_cont)
+          (H_tup:=SH_tup)
+          (lst:=(List.map run_cst_trans lst0)) 
+          (R:=[(ip,loc_w (next_cloc l));
+               (sp,loc_w (hloc L_out (List.length cur_stk_val)));
+               (nat_reg 1,val_direct_trans v cur_stk_val);
+               (nat_reg 2,o2);(nat_reg 3,o3);
+               (nat_reg 4,o4);(nat_reg 5,o5);(nat_reg 6,o6)])
+          (l:=next_cloc l) (P:=SC);automate;cbn.
+        - rewrite H15. inversion H11. cbn. 
+          assert (Temp:forall n, S n = n + 1).
+          { intros. rewrite PeanoNat.Nat.add_comm... }
+          rewrite Temp. apply app_nth2_plus with (n:=1) (l:=lst).
+        - destruct v as [cst|[ind|str]]... cbn. inversion H17...
+          inversion H5...
+        - inversion H13...
+          + inversion H2... specialize H1 with
+              (L_tup:=L_str) (vs:=lst0)... rewrite H20.
+          rewrite tuple_un_tuple... }
+      constructor. cbn.
+      apply S_push with (l:=incr_cloc 2 l) (lsp:=L_out)
+      (o:=reg_o (nat_reg 1)) (lst:=cur_stk_val)
+      (j:=List.length cur_stk_val) (H_stk:=cur_stkh) 
+      (H_cont:=SH_cont) (H_tup:=SH_tup)
+      (R:=[(ip,loc_w (incr_cloc 2 l));
+           (sp,loc_w (hloc L_out (List.length cur_stk_val)));
+           (nat_reg 1,nth i (un_tuple (SH_tup L_str)) ns);
+           (nat_reg 2,o2);(nat_reg 3,o3);(nat_reg 4,o4);
+           (nat_reg 5,o5);(nat_reg 6,o6)])... cbn.
+      rewrite H15. assert (Temp:forall n, S (S n) = n + 2).
+      { intros. rewrite PeanoNat.Nat.add_comm... } inversion H11.
+      rewrite Temp. apply app_nth2_plus with (n:=2) (l:=lst).
+    + (* prove LS_rel for L_get *)
+      unfold incr_cloc...
+      apply rel_LS with
+      (lst:=lst ++ firstn 3 SIlst)
+      (SIlst:= tl (tl (tl SIlst)));inversion H11...
+      * cbn. pose proof term_trans_not_nil as NN. specialize NN with
+          (tm:=t1'). destruct (RelConfig.LS.term_trans t1')as []eqn:?;automate.
+        rewrite <- Heql. rewrite <- PeanoNat.Nat.add_succ_comm.
+        apply rel_tm with (E:=nth (S i) lst0 L.ns :: E1) (t:=t1').
+      * apply rel_context with
+          (s:=s) (s_out:=s_out) (L_0:=L_0)...
+        rewrite <- map_nth with (d:=L.ns)...
+        inversion H13...
+        -- inversion H20... destruct i...
+        -- 
+
+          rewrite app_nth1...
+        
+        inversion H17... inversion H4...
+      * rewrite H15. cbn. assert (AssocIns: forall (x1:instr) x2 x3 x4 tl,
+          [x1;x2;x3;x4] ++ tl = x1::x2::x3::x4::tl). { intros... }
+        rewrite <- AssocIns,app_assoc_reverse...
+      * rewrite app_length. rewrite PeanoNat.Nat.add_comm...
+        
+    - (* x = v1 + v2 *) exists
+      ((L_out,stac  k ((int_w (i1+i2)) :: cur_stk_val))
         :: H_stack,SH_cont,SH_tup),
       ([(ip,loc_w (incr_cloc 4 l));(sp,loc_w (hloc L_out
         (1+(List.length cur_stk_val))));
@@ -238,10 +277,11 @@ Proof with automation.
       (R:=[(ip,loc_w (incr_cloc 3 l));(sp,loc_w (hloc L_out
         (List.length cur_stk_val)));(nat_reg 1,int_w (i1+i2));
         (nat_reg 2,int_w i2);(nat_reg 3,o3);(nat_reg 4,o4);
-        (nat_reg 5,o5);(nat_reg 6,o6)]);automation;simpl.
+        (nat_reg 5,o5);(nat_reg 6,o6)]);automate;simpl.
       rewrite H15. assert (Temp:forall n, S (S (S n)) = n + 3).
       { intros. rewrite PeanoNat.Nat.add_comm... } inversion H10...
       rewrite Temp. apply app_nth2_plus with (n:=3) (l:=lst).
+
     (* prove LS_rel for L_add *)
     + unfold h_update,incr_cloc,next_cloc... apply rel_LS with
       (lst:=lst ++ firstn 4 SIlst)
@@ -292,7 +332,7 @@ Proof with automation.
           (nat_reg 1,o1);(nat_reg 2,o2);(nat_reg 3,o3);
           (nat_reg 4,o4);(nat_reg 5,o5);(nat_reg 6,o6)])
           (l:=l) (P:=SC). rewrite PeanoNat.Nat.sub_diag in Ins.
-          apply Ins;automation;cbn.
+          apply Ins;automate;cbn.
           + inversion H10. rewrite H15... apply nth_middle.
           + rewrite h_eqb_refl... }
       constructor.
@@ -309,8 +349,9 @@ Proof with automation.
       inversion H10... rewrite Temp.
       apply app_nth2_plus with (n:=1) (l:=lst).
     + (* prove LS_rel for x=v *)
-      rewrite Heql. apply rel_LS with (lst:=lst ++ 
-        firstn 2 SIlst) (SIlst:= tl (tl SIlst))...
+      rewrite Heql. apply rel_LS with
+        (lst:=lst ++ firstn 2 SIlst) (SIlst:= tl (tl SIlst))...
+    
       * inversion H10. cbn. pose proof term_trans_not_nil as NN.
         specialize NN with (tm:=t1'). destruct
         (RelConfig.LS.term_trans t1')as []eqn:?... rewrite <- Heql.
